Add an interface with CompCert via the operator abstract layer : working example.

MinimpToClight.v
@@ -1,64 +1,25 @@
 Require Import Rustre.Minimp.Syntax.
 Require Import Rustre.Common.
 Require Import Rustre.Nelist.
-Require Import common.AST.
-Require Import common.Errors.
-Require Import cfrontend.Ctypes.
-Require Import cfrontend.Clight.
-Require Import cfrontend.Cop.
-Require Import lib.Integers.
-Require Import driver.Compiler.
+Require Import Rustre.Interface.
 
-Require Import ZArith.
-Open Scope string_scope.
+Module Import Syn := SyntaxFun Op.
+
+Require common.AST.
+Require common.Errors.
+Require cfrontend.Ctypes.
+Require cfrontend.Clight.
+Require cfrontend.Cop.
+Require driver.Compiler.
+
+Require Import String.
+
+(* Open Scope string_scope. *)
 Open Scope list_scope.
 Import List.ListNotations.
 
-Axiom pos_of_str : String.string -> ident.
-Axiom pos_to_str : ident -> String.string.
-
-Inductive unary_op' : Type :=
-| Opposite : unary_op'
-| Negation : unary_op'.
-Inductive binary_op' : Type :=
-| Plus : binary_op'
-| Minus : binary_op'
-| Mult : binary_op'.
-    
-Module Op <:
-  OPERATORS with Definition unary_op := unary_op'
-with Definition binary_op := binary_op'.
-    Definition val := Z.
-    Definition typ := Z.
-    Open Scope Z_scope.
-    Definition unary_op := unary_op'.
-    Definition binary_op := binary_op'.
-    Definition sem_unary (op : unary_op) (v : val) :=
-      match op with
-      | Opposite => Some (- v)
-      | Negation => Some (if Z.eqb v 0 then 1 else 0)
-      end.
-    Definition sem_binary (op : binary_op) (v1 v2 : val) :=
-      match op with
-      | Plus => Some (v1 + v2)
-      | Minus => Some (v1 - v2)
-      | Mult => Some (v1 * v2)
-      end.
-    Definition of_bool (b : bool) := if b then 1 else 0.
-    Definition to_bool n := match n with 0 => false | _ => true end.
-    Theorem bool_inv : forall b, to_bool (of_bool b) = b. Admitted.
-    Definition val_eqb := Z.eqb.
-    Definition unop_eqb (op1 op2 : unary_op) := true.
-    Definition binop_eqb (op1 op2 : binary_op) := true.
-    Theorem val_eqb_true_iff : forall v1 v2, val_eqb v1 v2 = true <-> v1 = v2. Admitted.
-    Theorem val_eqb_false_iff : forall v1 v2, val_eqb v1 v2 = false <-> v1 <> v2. Admitted.
-    Theorem unop_eqb_true_iff : forall op1 op2, unop_eqb op1 op2 = true <-> op1 = op2. Admitted.
-    Theorem unop_eqb_false_iff : forall op1 op2, unop_eqb op1 op2 = false <-> op1 <> op2. Admitted.
-    Theorem binop_eqb_true_iff : forall op1 op2, binop_eqb op1 op2 = true <-> op1 = op2. Admitted.
-    Theorem binop_eqb_false_iff : forall op1 op2, binop_eqb op1 op2 = false <-> op1 <> op2. Admitted.
-End Op.
-
-Module Import Syn := SyntaxFun Op.
+Axiom pos_of_str: String.string -> ident.
+Axiom pos_to_str: ident -> String.string.
 
 Definition example :=
   {|
@@ -72,88 +33,122 @@ Definition example :=
                                   (Syn.State (pos_of_str "t"))
                                   (Var (pos_of_str "i"))))
                    (AssignSt (pos_of_str "t") (Var (pos_of_str "o")));
-    c_reset := AssignSt (pos_of_str "t") (Const Z0)
+    c_reset := AssignSt (pos_of_str "t") (Const Vzero)
   |}.
 
+Definition cl_type := Ctypes.type.
+Definition cl_typelist := Ctypes.typelist.
+Definition cl_expr := Clight.expr.
+Definition cl_stmt := Clight.statement.
+Definition cl_bool := Ctypes.type_bool.
+Definition cl_int := Ctypes.type_int32s.
+Definition cl_ident := AST.ident.
+Definition cl_bind := prod cl_ident cl_type.
+Definition cl_globdef := AST.globdef Clight.fundef Ctypes.type.
+Definition cl_structdef := Ctypes.composite_definition.
+
 (** Common identifiers  *)
-Definition main_id : ident := pos_of_str "main".
-Definition step_id (id : ident) : ident := pos_of_str (String.append "step_" (pos_to_str id)).
-Definition reset_id (id : ident) : ident := pos_of_str (String.append "reset_" (pos_to_str id)).
-Definition self_id : ident := pos_of_str "self".
+Definition main_id: ident := pos_of_str "main".
+Definition step_id (id: cl_ident): ident :=
+  pos_of_str (String.append "step_" (pos_to_str id)).
+Definition reset_id (id: cl_ident): ident :=
+  pos_of_str (String.append "reset_" (pos_to_str id)).
+Definition self_id: ident := pos_of_str "self".
 
 (** struct types  *)
-Definition type_of_inst (o : ident) : type := Tstruct o noattr.
-Definition type_of_inst_p (o : ident) : type := Tpointer (type_of_inst o) noattr.
+Definition type_of_inst (o: cl_ident): cl_type :=
+  Ctypes.Tstruct o Ctypes.noattr.
+Definition type_of_inst_p (o: cl_ident): cl_type :=
+  Ctypes.Tpointer (type_of_inst o) Ctypes.noattr.
 
 (** Constants  *)
-Definition cl_true : expr := Econst_int Int.one type_bool.
-Definition cl_false : expr := Econst_int Int.zero type_bool.
-Definition cl_zero : expr := Econst_int Int.zero type_int32s.
+Definition cl_true: cl_expr := Clight.Econst_int one cl_bool.
+Definition cl_false: cl_expr := Clight.Econst_int zero cl_bool.
+Definition cl_zero: cl_expr := Clight.Econst_int zero cl_int.
 
-Definition translate_const (c : Op.val) : expr :=
-  Econst_int (Integers.Int.repr Z0) type_int32s.
+Definition translate_const (c: Op.val): cl_expr :=
+  Clight.Econst_int (Integers.Int.repr Z0) cl_int.
 
-Definition translate_type (ty : base_type) : type :=
+Definition translate_type (ty: base_type): cl_type :=
   match ty with
-  | Common.Tint => type_int32s
-  | Common.Tbool => type_bool
+  | Tint => cl_int
+  | Tbool => cl_bool
   end.
 
-Definition translate_unop (op : Op.unary_op) (e : expr) : expr :=
+Definition translate_unop (op: Op.unary_op) (e: cl_expr): cl_expr :=
   match op with
-  | Opposite => Eunop Oneg e type_int32s
-  | Negation => Eunop Onotbool e type_int32s
+  | Opposite => Clight.Eunop Cop.Oneg e cl_int
+  | Negation => Clight.Eunop Cop.Onotbool e cl_int
   end.
 
-Definition translate_binop (op : Op.binary_op) (e1 e2 : expr) : expr :=
+Definition translate_binop (op: Op.binary_op) (e1 e2: cl_expr): cl_expr :=
   match op with
-  | Plus => Ebinop Oadd e1 e2 type_int32s
-  | Minus => Ebinop Osub e1 e2 type_int32s
-  | Mult => Ebinop Omul e1 e2 type_int32s
+  | Plus => Clight.Ebinop Cop.Oadd e1 e2 cl_int
+  | Minus => Clight.Ebinop Cop.Osub e1 e2 cl_int
+  | Mult => Clight.Ebinop Cop.Omul e1 e2 cl_int
   end.
 
 (** Straightforward expression translation *)
-Fixpoint translate_exp (e : exp) : expr :=
+Fixpoint translate_exp (e: exp): cl_expr :=
   let ty := Common.Tint in
   match e with
-  | Syn.Var x (* ty *) => Evar x (translate_type ty)  
-  | Syn.State x (* ty *) => Evar x (translate_type ty) 
-  | Syn.Const c (* ty *) => translate_const c
-  | Syn.Unop op e (* ty *) =>
+  | Var x (* ty *) => Clight.Evar x (translate_type ty)  
+  | State x (* ty *) => Clight.Evar x (translate_type ty) 
+  | Const c (* ty *) => translate_const c
+  | Unop op e (* ty *) =>
     translate_unop op (translate_exp e)
-  | Syn.Binop op e1 e2 (* ty *) =>
+  | Binop op e1 e2 (* ty *) =>
     translate_binop op (translate_exp e1) (translate_exp e2)
   end.
 
-Fixpoint list_type_to_typelist (tys : list type) : typelist :=
+Fixpoint list_type_to_typelist (tys: list cl_type): cl_typelist :=
   match tys with
-  | [] => Tnil
-  | ty :: tys => Tcons ty (list_type_to_typelist tys)
+  | [] => Ctypes.Tnil
+  | ty :: tys => Ctypes.Tcons ty (list_type_to_typelist tys)
   end.
 
 (** pointer expressions  *)
-Definition pointer_of_cls (x cls : ident) : expr :=
-  Eaddrof (Evar x (type_of_inst cls)) (type_of_inst_p cls).
-(* Definition pointer_of_ty (x : ident) (ty : type) : expr := *)
-(*   Eaddrof (Evar x ty) (Tpointer ty noattr). *)
+Definition pointer_of_cls (x cls: cl_ident): cl_expr :=
+  Clight.Eaddrof (Clight.Evar x (type_of_inst cls)) (type_of_inst_p cls).
 
 (** function call and assignment *)
-(* Q : Can we really use same ident for temporary and classic variables ? *)
-Definition funcall (bind : option ident) (f : ident) (sig : type) (args : list expr) : statement :=
-  Scall bind (Evar f sig) args.
-Definition assign (bind : ident) (ty : type) (e : expr) : statement :=
-  Sassign (Evar bind ty) e.
-Definition binded_funcall (bind : ident) (f : ident) (ty : type) (args : list expr)
-  : (ident * type) * statement :=
+(* Q: Can we really use same ident for temporary and classic variables ? *)
+Definition funcall
+           (bind: option cl_ident) (f: cl_ident) (sig: cl_type)
+           (args: list cl_expr)
+  : cl_stmt :=
+  Clight.Scall bind (Clight.Evar f sig) args.
+
+Definition assign (bind: cl_ident) (ty: cl_type) (e: cl_expr): cl_stmt :=
+  Clight.Sassign (Clight.Evar bind ty) e.
+
+Definition st_assign (name x: cl_ident) (e: cl_expr): cl_stmt :=
+  let ty_self := type_of_inst_p name in
+  let ty_deref_self := type_of_inst name in
+  Clight.Sassign
+    (Clight.Efield (Clight.Ederef (Clight.Evar self_id ty_self) ty_deref_self) x
+                   (Clight.typeof e)) e.
+                 
+Definition binded_funcall (bind f: cl_ident) (ty: cl_type) (args: list cl_expr)
+  : cl_bind * cl_stmt :=
   let temp := bind in
-  let tys := List.map typeof args in
-  let sig := Tfunction (list_type_to_typelist tys) ty cc_default in
-  ((temp, ty), Ssequence (funcall (Some temp) f sig args) (assign bind ty (Etempvar temp ty))).
-Definition reset_call (cls : ident) (obj : ident) : statement :=
-  let ty_reset := Tfunction (Tcons (type_of_inst_p cls) Tnil) Tvoid cc_default in
+  let tys := List.map Clight.typeof args in
+  let sig := Ctypes.Tfunction (list_type_to_typelist tys) ty AST.cc_default in
+  ((temp, ty),
+   Clight.Ssequence (funcall (Some temp) f sig args)
+                    (assign bind ty (Clight.Etempvar temp ty))).
+
+Definition reset_call (cls obj: cl_ident): cl_stmt :=
+  let ty_reset :=
+      Ctypes.Tfunction (Ctypes.Tcons (type_of_inst_p cls) Ctypes.Tnil)
+                       Ctypes.Tvoid AST.cc_default
+  in
   funcall None (reset_id cls) ty_reset [pointer_of_cls obj cls].
-Definition step_call (bind : ident) (cls : ident) (obj : ident) (args : list expr) (out_ty : type)
-  : (ident * type) * statement :=
+
+Definition step_call
+           (bind cls: cl_ident) (obj: cl_ident) (args: list cl_expr)
+           (out_ty: cl_type)
+  : cl_bind * cl_stmt :=
   let args := pointer_of_cls obj cls :: args in
   binded_funcall bind (step_id cls) out_ty args.
 
@@ -161,21 +156,18 @@ Definition step_call (bind : ident) (cls : ident) (obj : ident) (args : list exp
 Statement conversion keeps track of the produced temporaries (function calls). 
 [name] represents the name of the current class.
  *)
-Fixpoint translate_stmt (temps : list (ident * type)) (name : ident) (s : stmt)
-  : (list (ident * type) * statement) :=
+Fixpoint translate_stmt (temps: list cl_bind) (name: cl_ident) (s: stmt)
+  : (list cl_bind * cl_stmt) :=
   match s with
   | Syn.Assign x e =>
     let ty := (* Syn.typeof e *) Common.Tint in
     (temps, assign x (translate_type ty) (translate_exp e))
   | Syn.AssignSt x e =>
-    let e' := translate_exp e in
-    let ty_self := type_of_inst_p name in
-    let ty_deref_self := type_of_inst name in
-    (temps, Sassign (Efield (Ederef (Evar self_id ty_self) ty_deref_self) x (typeof e')) e')
+    (temps, st_assign name x (translate_exp e))
   | Syn.Ifte e s1 s2 =>
     let (temps1, s1') := translate_stmt temps name s1 in
     let (temps2, s2') := translate_stmt temps1 name s2 in
-    (temps2, Sifthenelse (translate_exp e) s1' s2')
+    (temps2, Clight.Sifthenelse (translate_exp e) s1' s2')
   | Syn.Step_ap y cls x es (* ty *) =>
     let ty := Common.Tint in
     let args := nelist2list (Nelist.map translate_exp es) in
@@ -187,60 +179,76 @@ Fixpoint translate_stmt (temps : list (ident * type)) (name : ident) (s : stmt)
   | Syn.Comp s1 s2 =>
     let (temps1, s1') := translate_stmt temps name s1 in
     let (temps2, s2') := translate_stmt temps1 name s2 in
-    (temps2, Ssequence s1' s2')
+    (temps2, Clight.Ssequence s1' s2')
   | Syn.Skip =>
-    (temps, Sskip)
+    (temps, Clight.Sskip)
   end.
 
 (** return statements  *)
-Definition return_some (s : statement) (out : ident * type) : statement :=
+Definition return_some (s: cl_stmt) (out: cl_bind): cl_stmt :=
   let (id, ty) := out in
-  Ssequence s (Sreturn (Some (Evar id ty))).
-Definition return_none (s : statement) : statement :=
-  Ssequence s (Sreturn None).
-Definition return_zero (s : statement) : statement :=
-  Ssequence s (Sreturn (Some cl_zero)).
+  Clight.Ssequence s (Clight.Sreturn (Some (Clight.Evar id ty))).
+Definition return_none (s: cl_stmt): cl_stmt :=
+  Clight.Ssequence s (Clight.Sreturn None).
+Definition return_zero (s: cl_stmt): cl_stmt :=
+  Clight.Ssequence s (Clight.Sreturn (Some cl_zero)).
+
+Definition fundef
+           (ins: list cl_bind) (out: option cl_bind) (ty: cl_type)
+           (temps: list cl_bind) (body: cl_stmt)
+  : cl_globdef :=
+  let out := match out with Some o => [o] | None => [] end in 
+  let f := Clight.mkfunction ty AST.cc_default ins out temps body in
+  @AST.Gfun Clight.fundef cl_type (Clight.Internal f).
 
 (** build the step function *)
-Definition make_step (self : ident * type) (ins : list (ident * type))
-           (out : ident * type) (temps : list (ident * type)) (body : statement)
-  : globdef fundef type :=
+Definition make_step
+           (self: cl_bind) (ins: list cl_bind) (out: cl_bind)
+           (temps: list cl_bind) (body: cl_stmt)
+  : cl_globdef :=
   let body := return_some body out in
-  let f := mkfunction (snd out) cc_default (self :: ins) [out] temps body in
-  @Gfun fundef type (Internal f).
+  fundef (self :: ins) (Some out) (snd out) temps body.
 
-Fixpoint seq_of_statements (sl: list statement) : statement :=
+Fixpoint seq_of_statements (sl: list cl_stmt): cl_stmt :=
   match sl with
-  | [] => Sskip
-  | s :: sl' => Ssequence s (seq_of_statements sl')
+  | [] => Clight.Sskip
+  | s :: sl' => Clight.Ssequence s (seq_of_statements sl')
   end.
 
-Definition reset_obj (obj : obj_dec) : statement :=
+Definition reset_obj (obj: obj_dec): cl_stmt :=
   reset_call (obj_class obj) (obj_inst obj).
 
 (** build the reset function *)
-Definition make_reset (self : ident * type) (objs : list obj_dec)
-           (temps : list (ident * type)) (body : statement) : globdef fundef type :=
+Definition make_reset
+           (self: cl_bind) (objs: list obj_dec) (temps: list cl_bind)
+           (body: cl_stmt)
+  : cl_globdef :=
   let seq_res := seq_of_statements (body :: (List.map reset_obj objs)) in
   let body := return_none seq_res in
-  let f := mkfunction Tvoid cc_default [self] [] temps body in
-  @Gfun fundef type (Internal f).
+  fundef [self] None Ctypes.Tvoid temps body.
 
-Definition translate_obj_dec (obj : obj_dec) : (ident * type) :=
-  match obj with mk_obj_dec inst cls => (inst, type_of_inst cls) end.
+Definition translate_ident (id: ident): cl_ident := id.
 
-Definition translate_param (p : ident (* * base_type *)) : (ident * type) :=
+Definition translate_obj_dec (obj: obj_dec): cl_bind :=
+  match obj with
+    mk_obj_dec inst cls =>
+    let inst := translate_ident inst in
+    let cls := translate_ident cls in
+    (inst, type_of_inst cls)
+  end.
+
+Definition translate_param (p: ident): cl_bind :=
   let (id, ty) := (p, Common.Tint) in
-  (id, translate_type ty).
+  (translate_ident id, translate_type ty).
 
 (** build the structure *)
-Definition make_struct (name : ident) (members : list (ident * type))
-  : composite_definition :=
-  Composite name Struct members noattr.
+Definition make_struct (name: cl_ident) (members: list cl_bind)
+ : cl_structdef :=
+  Ctypes.Composite name Ctypes.Struct members Ctypes.noattr.
 
-(** translate a class into a triple : structure, step function, reset function  *)
-Definition translate_class (c : Syn.class)
-  : composite_definition * (ident * globdef fundef type) * (ident * globdef fundef type) :=
+(** translate a class into a triple: structure, step function, reset function  *)
+Definition translate_class (c: class)
+ : cl_structdef * (cl_ident * cl_globdef) * (cl_ident * cl_globdef) :=
   match c with
     mk_class c_name c_input c_output c_mems c_objs c_step c_reset =>
     let mems := List.map translate_param c_mems in
@@ -248,30 +256,31 @@ Definition translate_class (c : Syn.class)
     let ins := nelist2list (Nelist.map translate_param c_input) in
     let out := translate_param c_output in
     let members := mems ++ objs in
-    let (temps_step, step) := translate_stmt [] c_name c_step in
-    let (temps_reset, reset) := translate_stmt [] c_name c_reset in
-    let self := (self_id, type_of_inst_p c_name) in
-    let cl_struct := make_struct c_name members in
-    let cl_step := (step_id c_name, make_step self ins out temps_step step) in
-    let cl_reset := (reset_id c_name, make_reset self c_objs temps_reset reset) in
+    let name := translate_ident c_name in
+    let (temps_step, step) := translate_stmt [] name c_step in
+    let (temps_reset, reset) := translate_stmt [] name c_reset in
+    let self := (self_id, type_of_inst_p name) in
+    let cl_struct := make_struct name members in
+    let cl_step := (step_id name, make_step self ins out temps_step step) in
+    let cl_reset := (reset_id name, make_reset self c_objs temps_reset reset) in
     (cl_struct, cl_step, cl_reset) 
   end.
 
 (** build the main function (entry point) *)
-Definition make_main (node : ident) (f : ident) (ins : nelist ident) (out : ident)
-  : globdef fundef type :=
+Definition make_main
+           (node: cl_ident) (f: cl_ident) (ins: nelist cl_ident) (out: cl_ident)
+ : cl_globdef :=
   let ty := Common.Tint in
   let args := nelist2list (Nelist.alls cl_zero ins) in
   let out_ty := translate_type ty in
   let (temp, step) := step_call out node f args out_ty in
-  let loop := Swhile cl_true step in
-  let body := return_zero (Ssequence (reset_call node f) loop) in
-  let f := mkfunction type_int32s cc_default [] [] [temp] body in 
-  @Gfun fundef type (Internal f).
+  let loop := Clight.Swhile cl_true step in
+  let body := return_zero (Clight.Ssequence (reset_call node f) loop) in
+  fundef [] None cl_int [temp] body.
 
-Definition split_3 {A B C : Type} (l : list (A * B * C))
-  : list A * list B * list C :=
-  List.fold_right (fun (xyz : A * B * C) (abc : list A * list B * list C) =>
+Definition split_3 {A B C: Type} (l: list (A * B * C))
+ : list A * list B * list C :=
+  List.fold_right (fun (xyz: A * B * C) (abc: list A * list B * list C) =>
                      match xyz with
                        (x, y, z) => match abc with
                                      (a, b, c) => (x :: a, y :: b, z :: c)
@@ -279,27 +288,35 @@ Definition split_3 {A B C : Type} (l : list (A * B * C))
                      end
                   ) ([], [], []) l.
 
-(** translation function : the main instance is declared as 'extern' and it's step function's return 
-variable as 'volatile' *)
-Definition translate (p : Syn.program) (main_node : ident) : res Clight.program :=
+Definition vardef (ty: cl_type) (volatile: bool): cl_globdef :=
+  @AST.Gvar Clight.fundef cl_type (AST.mkglobvar ty [] false volatile).
+
+(** translation function: the main instance is declared as 'extern' and it's 
+step function's return variable as 'volatile' *)
+Definition translate (p: program) (main_node: ident)
+  : Errors.res Clight.program :=
+  let main_node := translate_ident main_node in
   match find_class main_node p with
   | Some (cls, _) =>
     let f := pos_of_str "f_" in
     let o := pos_of_str "o_" in
-    let f_gvar := @Gvar fundef type (mkglobvar (type_of_inst main_node) nil false false) in
-    let o_gvar := @Gvar fundef type (mkglobvar type_int32s nil false true) in
+    let f_gvar := vardef (type_of_inst main_node) false in
+    let o_gvar := vardef cl_int true in
     let main := make_main main_node f (c_input cls) o in
     let cs := List.map translate_class p in
     match split_3 cs with
       (structs, steps, resets) =>
-      let gdefs := (o, o_gvar) :: (f, f_gvar) :: resets ++ steps ++ [(main_id, main)] in
-      make_program structs gdefs [] main_id                    
+      let gdefs := (o, o_gvar) :: (f, f_gvar) ::
+                               resets ++ steps ++ [(main_id, main)]
+      in
+      Clight.make_program structs gdefs [] main_id                    
     end
-  | None => Error (msg "undefined node")
+  | None => Errors.Error (Errors.msg "undefined node")
   end. 
 
-Definition compile (p : Syn.program) (main_node : ident) : res Asm.program :=
+Definition compile (p: Syn.program) (main_node: cl_ident)
+  : Errors.res Asm.program :=
   match translate p main_node with
-  | OK p => transf_clight_program p
-  | Error res => Error res
+  | Errors.OK p => Compiler.transf_clight_program p
+  | Errors.Error res => Errors.Error res
   end.
