Interface.v
@@ -1,0 +1,125 @@
+Require Import compcert.lib.Integers.
+Require Import Rustre.Common.
+
+(* Interface avec CompCert *)
+Inductive val' : Type :=
+| Vundef : val'
+| Vint : Int.int -> val'. 
+Inductive unary_op' : Type :=
+| Opposite : unary_op'
+| Negation : unary_op'.
+Inductive binary_op' : Type :=
+| Plus : binary_op'
+| Minus : binary_op'
+| Mult : binary_op'.
+
+Definition zero := Int.zero.
+Definition one := Int.one.
+Definition Vzero := Vint Int.zero.
+
+Module Op <: OPERATORS.
+  Definition val := val'.
+  Definition typ := nat.
+  
+  Definition unary_op := unary_op'.
+  Definition binary_op := binary_op'.
+
+  Definition sem_opposite (v : val) : option val :=
+    match v with
+    | Vundef => None
+    | Vint n => Some (Vint (Int.neg n))
+    end.
+
+  Definition sem_negation (v : val) : option val :=
+    match v with
+    | Vundef => None
+    | Vint n => Some (Vint (if (Int.eq n zero) then one else zero))
+    end.
+  
+  Definition sem_unary (op : unary_op) (v : val) : option val :=
+    match op with
+    | Opposite => sem_opposite v
+    | Negation => sem_negation v
+    end.
+
+  Definition sem_plus (v1 v2 : val) : option val :=
+    match v1, v2 with
+    | Vint n1, Vint n2 => Some (Vint (Int.add n1 n2))
+    | _, _ => None
+    end.
+
+  Definition sem_minus (v1 v2 : val) : option val :=
+    match v1, v2 with
+    | Vint n1, Vint n2 => Some (Vint (Int.sub n1 n2))
+    | _, _ => None
+    end.
+
+  Definition sem_mult (v1 v2 : val) : option val :=
+    match v1, v2 with
+    | Vint n1, Vint n2 => Some (Vint (Int.mul n1 n2))
+    | _, _ => None
+    end.
+  
+  Definition sem_binary (op : binary_op) (v1 v2 : val) : option val :=
+    match op with
+    | Plus => sem_plus v1 v2
+    | Minus => sem_minus v1 v2
+    | Mult => sem_mult v1 v2
+    end.
+
+  Definition of_bool (b : bool) : val := Vint (if b then Int.one else Int.zero).
+  Definition to_bool (v : val) : bool :=
+    match v with
+    | Vundef => false
+    | Vint n => negb (Int.eq n Int.zero)
+    end.
+
+  Theorem bool_inv : forall b : bool, to_bool (of_bool b) = b. 
+  Proof. now destruct b. Qed.
+
+  Lemma val_dec : forall v1 v2 : val, {v1 = v2} + {v1 <> v2}.
+  Proof. decide equality; apply Int.eq_dec. Qed.
+  Definition val_eqb (v1 v2 : val) : bool :=
+    match v1, v2 with
+    | Vundef, Vundef => true
+    | Vint n1, Vint n2 => Int.eq n1 n2
+    | _, _ => false
+    end.
+
+  Lemma unop_dec : forall op1 op2 : unary_op, {op1 = op2} + {op1 <> op2}.
+  Proof. decide equality. Qed.
+  Definition unop_eqb (op1 op2 : unary_op) := if unop_dec op1 op2 then true else false.
+
+  Lemma binop_dec : forall op1 op2 : binary_op, {op1 = op2} + {op1 <> op2}.
+  Proof. decide equality. Qed.
+  Definition binop_eqb (op1 op2 : binary_op) := if binop_dec op1 op2 then true else false.
+  
+  Theorem val_eqb_true_iff : forall v1 v2, val_eqb v1 v2 = true <-> v1 = v2.
+  Proof.
+    intros v1 v2; unfold val_eqb; destruct v1 as [|n1], v2 as [|n2]; try intuition discriminate.
+    split; intro H.
+    - pose proof (Int.eq_spec n1 n2) as Heq; rewrite H in Heq; now f_equal.
+    - inversion H; apply Int.eq_true.
+  Qed.
+
+  Theorem val_eqb_false_iff : forall v1 v2, val_eqb v1 v2 = false <-> v1 <> v2.
+  Proof.
+    intros v1 v2; unfold val_eqb; destruct v1 as [|n1], v2 as [|n2]; try intuition discriminate.
+    split; intros H.
+    - intro Hf; pose proof (Int.eq_spec n1 n2) as Hneq; rewrite H in Hneq; inversion Hf as [Heq]; contradiction. 
+    - apply Int.eq_false; intro Heq; apply H; now f_equal.
+  Qed.
+
+  Theorem unop_eqb_true_iff : forall op1 op2, unop_eqb op1 op2 = true <-> op1 = op2.
+  Proof. intros op1 op2; unfold unop_eqb; destruct (unop_dec op1 op2); intuition discriminate. Qed.
+  
+  Theorem unop_eqb_false_iff : forall op1 op2, unop_eqb op1 op2 = false <-> op1 <> op2.
+  Proof. intros op1 op2; unfold unop_eqb; destruct (unop_dec op1 op2); intuition. Qed.
+
+  Theorem binop_eqb_true_iff : forall op1 op2, binop_eqb op1 op2 = true <-> op1 = op2. 
+  Proof. intros op1 op2; unfold binop_eqb; destruct (binop_dec op1 op2); intuition discriminate. Qed.
+  
+  Theorem binop_eqb_false_iff : forall op1 op2, binop_eqb op1 op2 = false <-> op1 <> op2. 
+  Proof. intros op1 op2; unfold binop_eqb; destruct (binop_dec op1 op2); intuition. Qed.
+
+End Op.
